Stuff

ling.v
@@ -1,48 +1,144 @@
 Require Import Bool Arith List.
 Require Import Coq.Program.Equality.
 Require Import Program.
-Load hlist.
-Load syntax.
 Set Implicit Arguments.
 Set Asymmetric Patterns.
 
+(* Adam Chlipalas heterogeneous list implementation (magic inside)
+ * Useful for De Bruijn indices
+ *)
+
+Section hlist.
+  Variable A : Type.
+  Variable B : A -> Type.
+
+  Inductive hlist : list A -> Type :=
+  | HNil : hlist nil
+  | HCons : forall (x : A) (ls : list A), B x -> hlist ls -> hlist (x :: ls).
+
+  Variable elm : A.
+
+  Inductive member : list A -> Type :=
+  | HFirst : forall ls, member (elm :: ls)
+  | HNext : forall x ls, member ls -> member (x :: ls).
+
+  Fixpoint hget ls (mls : hlist ls) : member ls -> B elm :=
+    match mls with
+    | HNil
+      => fun mem =>
+           match mem in member ls'
+                 return (match ls' with
+                         | nil => B elm
+                         | _ :: _ => unit
+                         end) with
+           | HFirst _ => tt
+           | HNext _ _ _ => tt
+           end
+    | HCons _ _ x mls'
+      => fun mem =>
+           match mem in member ls'
+                 return (match ls' with
+                         | nil => Empty_set
+                         | x' :: ls'' =>
+                           B x' -> (member ls'' -> B elm)
+                           -> B elm
+                         end) with
+           | HFirst _ => fun x _ => x
+           | HNext _ _ mem' => fun _ get_mls' => get_mls' mem'
+           end x (hget mls')
+    end.
+  
+End hlist.
+
+Arguments HNil [A B].
+Arguments HCons [A B x ls].
+
+Arguments HFirst [A elm ls].
+Arguments HNext [A elm x ls].
+
+Inductive ty : Type :=
+| TBool : ty
+| TNat : ty
+| TList : ty -> ty.
+
+Definition env := list ty.
+
+(* Intrinsically typed expression syntax *)
+Inductive exp G : ty -> Type :=
+| evar : forall t, member t G -> exp G t
+| etrue : exp G TBool
+| efalse : exp G TBool
+| econst : nat -> exp G TNat
+| esucc : exp G TNat -> exp G TNat
+| enil : forall t, exp G (TList t)
+| econs : forall t, exp G t -> exp G (TList t) -> exp G (TList t)
+| elet : forall t1 t2, exp G t1 -> exp (t1 :: G) t2 -> exp G t2
+| eappend : forall t, exp G (TList t) -> exp G (TList t) -> exp G (TList t)
+| emap : forall t1 t2, exp (t1 :: G) t2 -> exp G (TList t1) -> exp G (TList t2)
+| efilter : forall t1, exp (t1 :: G) TBool -> exp G (TList t1) -> exp G (TList t1).
+
+Arguments econst [G].
+Arguments etrue [G].
+Arguments efalse [G].
+Arguments enil [G t].
+
+Notation "[| |]" := enil.
+Notation "[| x |]" := (econs x enil).
+Notation "[| x ; y ; .. ; z |]" := (econs x (econs y .. (econs z enil) ..)).
+Notation "[| x ; .. ; y |]" := (econs x .. (econs y enil) ..).
+
+(* Intrinsically typed values as well *)
+Inductive val : ty -> Type :=
+| vtrue : val TBool
+| vfalse : val TBool
+| vconst : nat -> val TNat
+| vnil : forall t, val (TList t)
+| vcons : forall t, val t -> val (TList t) -> val (TList t).
+
+Notation "[|| ||]" := vnil.
+Notation "[|| x ||]" := (vcons x vnil).
+Notation "[|| x ; y ; .. ; z ||]" := (vcons x (vcons y .. (vcons z vnil) ..)).
+Notation "[|| x ; .. ; y ||]" := (vcons x .. (vcons y vnil) ..).
+
 Example inc : exp nil (TList TNat) :=
-  emap (eplus (evar zvar) (econst 3)) (econs (econst 4) enil).
+  emap (esucc (evar HFirst)) (econs (econst 4) enil).
 
 Example let_ex : exp nil TNat :=
-  elet (econst 42) (eplus (evar zvar) (econst 10)).
+  elet (econst 42) (esucc (evar HFirst)).
 
 Example app_prog : exp nil (TList TNat) := eappend (econs (econst 0) enil) (econs (econst 1) enil).
 
 Example nested_map : exp nil (TList TNat) :=
-  emap (eplus (econst 3) (evar zvar))
-  (emap (eplus (evar zvar) (econst 10)) [| econst 1 ; econst 2 ; econst 3 |]).
+  emap (esucc (evar HFirst))
+  (emap (esucc (evar HFirst)) [| econst 1 ; econst 2 ; econst 3 |]).
 
 Example flat_map : exp nil (TList TNat) :=
-  emap (eplus (econst 3) (eplus (evar zvar) (econst 10)))
+  emap (esucc (esucc (evar HFirst)))
        [| econst 1 ; econst 2 ; econst 3 |].
 
-Definition Sub G G' := forall t, var G t -> exp G' t. 
+Definition Sub G G' := forall t, member t G -> exp G' t. 
 
 Definition idSub {G} : Sub G G := @evar G.
 
 Program Definition consSub {G G' t} (e:exp G' t) (s:Sub G G') : Sub (t::G) G' :=
-  fun t' (v: var (t::G) t') =>
+  fun t' (v: member t' (t::G)) =>
     match v with
-    | zvar _ _ => e
-    | svar _ _ _ v' => s _ v'
+    | HFirst _ => e
+    | HNext _ _ v' => s _ v'
     end.
     
 Notation "{| e ; .. ; f |}" := (consSub e .. (consSub f idSub) ..).
 
-Definition Ren G G' := forall t, var G t -> var G' t.
+Check @member.
+
+Definition Ren G G' := forall t, @member ty t G -> @member ty t G'.
 
 Program Definition renameLift {G G' t}
         (r : Ren G G') : Ren (t :: G) (t :: G') :=
   fun t' v =>
     match v with
-    | zvar _ _ => zvar
-    | svar _ _ _ v' => svar (r _ v')
+    | HFirst _ => @HFirst ty t _
+    | HNext _ _ v' => HNext (r _ v')
     end.
 
 Fixpoint renameExp G G' t (r : Ren G G') (e : exp G t) :=
@@ -51,7 +147,7 @@ Fixpoint renameExp G G' t (r : Ren G G') (e : exp G t) :=
   | etrue => etrue
   | efalse => efalse
   | econst n => econst n
-  | eplus e1 e2 => eplus (renameExp r e1) (renameExp r e2)
+  | esucc e => esucc (renameExp r e)
   | enil _ => enil
   | econs _ e1 e2 => econs (renameExp r e1) (renameExp r e2)
   | elet _ _ e1 e2 => elet (renameExp r e1) (renameExp (renameLift r) e2)
@@ -61,14 +157,14 @@ Fixpoint renameExp G G' t (r : Ren G G') (e : exp G t) :=
   end.
 
 Definition shiftExp G t t' : exp G t -> exp (t' :: G) t :=
-  renameExp (fun _ v => svar v).
+  renameExp (fun _ v => HNext v).
 
 Program Definition
         subShift {G G'} t (s : Sub G G') : Sub (t :: G) (t :: G') :=
   fun t' v =>
     match v with
-    | zvar _ _ => evar zvar
-    | svar _ _ _ v' => shiftExp t (s _ v')
+    | HFirst _ => evar HFirst
+    | HNext _ _ v' => shiftExp t (s _ v')
     end.
 
 Fixpoint subExp G G' t (s : Sub G G') (e : exp G t) :=
@@ -77,7 +173,7 @@ Fixpoint subExp G G' t (s : Sub G G') (e : exp G t) :=
   | etrue => etrue
   | efalse => efalse
   | econst n => econst n
-  | eplus e1 e2 => eplus (subExp s e1) (subExp s e2)
+  | esucc e => esucc (subExp s e)
   | enil _ => enil
   | econs _ e1 e2 => econs (subExp s e1) (subExp s e2)
   | elet _ _ e1 e2 => elet (subExp s e1) (subExp (subShift s) e2)
@@ -108,37 +204,30 @@ Fixpoint envDenote G : Type :=
   | t :: G => prodT (tyDenote t) (envDenote G)
   end.
 
-Fixpoint getVar G t (v : var G t) : envDenote G -> tyDenote t :=
-  match v with
-  | zvar _ _ => fun se => fst se
-  | svar _ _ _ v => fun se => getVar v (snd se)
-  end.
-
 (* An interpreter *)
-Fixpoint expDenote G t (e : exp G t) : envDenote G -> tyDenote t :=
+Fixpoint expDenote G t (e : exp G t) : hlist tyDenote G -> tyDenote t :=
   match e with
-  | evar _ x => getVar x
+  | evar _ x => fun s => hget s x 
   | econst n => fun _ => n
   | etrue => fun _ => true
   | efalse => fun _ => false
-  | eplus e1 e2 => fun s => (expDenote e1 s) + (expDenote e2 s)
+  | esucc e => fun s => S (expDenote e s)
   | enil _ => fun _ => nil
   | econs _ e1 e2 => fun s => (expDenote e1 s) :: (expDenote e2 s)
   | elet _ _ e el =>
-    fun s => expDenote el ((expDenote e s), s)
+    fun s => expDenote el (HCons (expDenote e s) s)
   | eappend _ e1 e2 => fun s => app (expDenote e1 s) (expDenote e2 s)
   | emap _ _ ef e =>
-    fun s => let f := fun x => expDenote ef (x, s)
+    fun s => let f := fun x => expDenote ef (HCons x s)
              in map f (expDenote e s)
   | efilter _ ef e =>
-    fun s => let f := fun x => expDenote ef (x, s)
+    fun s => let f := fun x => expDenote ef (HCons x s)
              in filter f (expDenote e s)
   end.
 
-Eval compute in (expDenote app_prog) ().
-Eval compute in (expDenote let_ex) ().
-Eval compute in (expDenote inc) ().
-
+Eval compute in (expDenote app_prog) HNil.
+Eval compute in (expDenote let_ex) HNil.
+Eval compute in (expDenote inc) HNil.
 
 Lemma append_assoc : forall G t (e1 e2 e3: exp G (TList t)) s,
     expDenote (eappend (eappend e1 e2) e3) s =
@@ -159,21 +248,69 @@ Qed.
  * replace all occurences of x in f by result of g
  *)
 
-Print nested_map.
+Definition tlSub {G G' t} (s : Sub (t :: G) G') : Sub G G' :=
+  fun t' v => s t' (HNext v).
 
-Eval simpl in subExp {| econst 10; econst 20 |} (eplus (evar zvar) (evar (svar zvar))).
+Definition hdSub {G G' t} (s : Sub (t :: G) G') : exp G' t :=
+  s t HFirst.
 
-Example nested_map' : exp nil (TList TNat) :=
-  emap (eplus (econst 3) (evar zvar))
-  (emap (eplus (evar zvar) (econst 10)) [| econst 1 ; econst 2 ; econst 3 |]).
+Definition ty_ctx := list ty.
+Definition ev_ctx G := hlist val G.
 
-Example f1 : exp (TNat :: nil) (TList TNat) := (econs (evar zvar) enil).
-Example f2 : exp (TNat :: nil) TNat := (eplus (evar zvar) (econst 10)).
+Fixpoint insertAt (t : ty) (G : ty_ctx) (n : nat) {struct n} : ty_ctx :=
+  match n with
+  | O => t :: G
+  | S n' => match G with
+            | nil => t :: G
+            | t' :: G' => t' :: insertAt t G' n'
+            end
+  end.
 
-Check (subExp {| f2 |} (shiftExp _ f1)).
+Fixpoint liftVar t G (x : member t G) t' n
+  : member t (insertAt t' G n) :=
+  match x with
+  | HFirst G' => match n return member t (insertAt t' (t :: G') n) with
+                 | O => HNext HFirst
+                 | _ => HFirst
+                 end
+  | HNext t'' G' x' => match n return member t (insertAt t' (t'' :: G') n) with
+                       | O => HNext (HNext x')
+                       | S n' => HNext (liftVar x' t' n')
+                       end
+  end.
 
-Eval simpl in expDenote (emap f1 (emap f2 [| econst 10; econst 20; econst 30 |])).
-Eval simpl in expDenote (emap (subExp {| f2 |} (shiftExp _ f1)) [| econst 10; econst 20; econst 30 |]).
+Fixpoint lift' G t' n t (e : exp G t) : exp (insertAt t' G n) t :=
+  match e with
+  | evar _ x => evar (liftVar x t' n)
+  | econst n => econst n
+  | etrue => etrue
+  | efalse => efalse
+  | esucc e => esucc (lift' t' n e)
+  | enil _ => enil
+  | econs _ e1 e2 => econs (lift' t' n e1) (lift' t' n e2)
+  | elet _ _ e1 e2 => elet (lift' t' n e1) (lift' t' (S n) e2)
+  | eappend _ e1 e2 => eappend (lift' t' n e1) (lift' t' n e2)
+  | emap _ _ e1 e2 => emap (lift' t' (S n) e1) (lift' t' n e2)
+  | efilter _ e1 e2 => efilter (lift' t' (S n) e1) (lift' t' n e2)
+  end.
+
+Definition lift G t' t (e : exp G t) : exp (t' :: G) t :=
+  lift' t' O e.
+
+Definition compose t1 t2 t3 G (f : exp (t1 :: G) t2) (g : exp (t2 :: G) t3) : exp (t1 :: G) t3 :=
+  subExp {| f |} (lift' t1 (S O) g).
+
+
+(* Program Definition map_fusion t G (e : exp G (TList t)) :=
+  match e in exp _ (TList t) return exp G (TList t) with
+  | emap t2 t g em => match em in exp _ (TList t1) return exp G (TList t) with
+                       | emap t1 t2 f eb => emap (compose f g) eb
+                       | _ => emap g em
+                       end
+  |  _ => e
+  end.
+*)
+  
 
 (* Inductive judgment for append *)
 Inductive CApp : forall t,
@@ -182,30 +319,76 @@ Inductive CApp : forall t,
 | CAppCons : forall t v (v1 : val t) v2 v3,
     CApp v2 v3 v -> CApp (vcons v1 v2) v3 (vcons v1 v).
 
-(* The beginning of an inductive judgment for map
- * This may need to be mutally inductive with Ev
- *)
-Inductive CMap : forall G t1 t2,
-    val (TList t1) -> exp G t2 -> val (TList t2) -> Prop :=
-| CMapNil : forall G t1 t2 (e : exp G t2), CMap (vnil t1) e (vnil t2).
+Inductive Ev : forall G t, ev_ctx G -> exp G t -> val t -> Prop :=
+| EvVar : forall G R t (m : member t G),
+    Ev R (evar m) (hget R m)
+| EvTrue : forall (G : ty_ctx) (R : ev_ctx G),
+    Ev R etrue vtrue
+| EvFalse : forall (G : ty_ctx) (R : ev_ctx G),
+    Ev R efalse vfalse
+| EvConst : forall (G : ty_ctx) (R : ev_ctx G) n,
+    Ev R (econst n) (vconst n)
+| EvNil : forall (G : ty_ctx) (R : ev_ctx G) t,
+    Ev R enil (vnil t)
+| EvCons : forall (G : ty_ctx) (R : ev_ctx G)
+                  t e1 e2 (v1 : val t) (v2 : val (TList t)),
+    Ev R e1 v1 -> Ev R e2 v2 -> Ev R (econs e1 e2) (vcons v1 v2)
+| EvAppend : forall (G : ty_ctx) (R : ev_ctx G) t
+                    (e1 e2 : exp G (TList t)) (v1 v2 : val (TList t)) v,
+    Ev R e1 v1 -> Ev R e2 v2 ->
+    CApp v1 v2 v -> Ev R (eappend e1 e2) v
+| EvSucc : forall (G : ty_ctx) (R : ev_ctx G) e n,
+    Ev R e (vconst n) -> Ev R (esucc e) (vconst (S n))
+| EvLet : forall (G : ty_ctx) (R : ev_ctx G)
+                 t1 t2 (e1 : exp G t1) (e2 : exp (t1 :: G) t2) v1 (v2 : val t2),
+    Ev R e1 v1 -> Ev (HCons v1 R) e2 v2 -> Ev R (elet e1 e2) v2
+| EvMap : forall (G : ty_ctx) (R : ev_ctx G) t1 t2
+                 (e1 : exp (t1 :: G) t2) (e2 : exp G (TList t1)) v v',
+                 Ev R e2 v ->
+                 CMap R v e1 v' ->
+                 Ev R (emap e1 e2) v'
+ with CMap : forall G t1 t2,
+    ev_ctx G -> val (TList t1) -> exp (t1 :: G) t2 -> val (TList t2) -> Prop :=
+      | CMapNil : forall (G : ty_ctx) (R : ev_ctx G) t1 t2 (e : exp (t1 :: G) t2),
+          CMap R (vnil t1) e (vnil t2)
+      | CMapCons : forall (G : ty_ctx) (R : ev_ctx G) t1 t2 (e : exp (t1 :: G) t2)
+        v1 v2 v1' v2',
+          Ev (HCons v1 R) e v1' ->
+          CMap R v2 e v2' ->
+          CMap R (vcons v1 v2) e (vcons v1' v2')
+ with CFilter : forall G t,
+     ev_ctx G -> val (TList t) -> exp (t :: G) TBool -> val (TList t) -> Prop :=
+      | CFilterNil : forall (G : ty_ctx) (R : ev_ctx G) t (e : exp (t :: G) TBool),
+          CFilter R (vnil t) e (vnil t)
+      | CFilterTrue : forall (G : ty_ctx) (R : ev_ctx G) t (e : exp (t :: G) TBool) v1 v2 v2',
+          Ev (HCons v1 R) e vtrue ->
+          CFilter R v2 e v2' ->
+          CFilter R (vcons v1 v2) e (vcons v1 v2')
+      | CFilterFalse : forall (G : ty_ctx) (R : ev_ctx G) t (e : exp (t :: G) TBool) v1 v2 v2',
+          Ev (HCons v1 R) e vfalse ->
+          CFilter R v2 e v2' ->
+          CFilter R (vcons v1 v2) e v2'.
 
-(* The start of an inductive evaluation relation *)
-Inductive Ev : forall t, exp nil t -> val t -> Prop :=
-| EvTrue : Ev etrue vtrue
-| EvFalse : Ev efalse vfalse
-| EvConst : forall n, Ev (econst n) (vconst n)
-| EvNil : forall t, Ev enil (vnil t)
-| EvCons : forall t (e1 : exp nil t) (e2 : exp nil (TList t))
-                  (v1 : val t) (v2 : val (TList t)),
-    Ev e1 v1 -> Ev e2 v2 -> Ev (econs e1 e2) (vcons v1 v2)
-| EvAppend : forall t (e1 : exp nil (TList t)) (e2 : exp nil (TList t)) v1 v2 v,
-    Ev e1 v1 -> Ev e2 v2 -> CApp v1 v2 v -> Ev (eappend e1 e2) v
-| EvPlus : forall (e1 e2 : exp nil TNat) n1 n2,
-    Ev e1 (vconst n1) -> Ev e2 (vconst n2) -> Ev (eplus e1 e2) (vconst (n1 + n2)).
+Scheme Ev_mut := Induction for Ev Sort Prop
+                 with CMap_mut := Induction for CMap Sort Prop
+                                  with CFilter_mut := Induction for CFilter Sort Prop.
+
+Check Ev_mut.
 
 Example ev_example :
-  Ev etrue vtrue.
-apply EvTrue.
+  Ev (HCons (vconst 1) HNil) (evar HFirst) (vconst 1).
+apply EvVar.
+Qed.
+
+Example ev_let :
+  Ev HNil (elet (econst 10) (esucc (evar HFirst))) (vconst 11).
+repeat econstructor.
+Qed.
+
+Example ev_map :
+  Ev HNil (emap (esucc (evar HFirst)) [| econst 10 ; econst 11 |])
+     (vcons (vconst 11) (vcons (vconst 12) (vnil TNat))).
+repeat econstructor.
 Qed.
 
 (* CApp is deterministic *)
@@ -222,9 +405,14 @@ Proof.
   assumption.
 Qed.
 
+Lemma vconst_congS : forall n n0, vconst n = vconst n0 -> vconst (S n) = vconst (S n0).
+  Proof.
+    intros.
+    congruence.
+Qed.
 (* Evaluation relation is deterministic *)
-Lemma ev_determ : forall t (e: exp nil t) v1 v2,
-    Ev e v1 -> Ev e v2 -> v1 = v2.
+Lemma ev_determ : forall G (R : ev_ctx G) t (e: exp G t) v1 v2,
+    Ev R e v1 -> Ev R e v2 -> v1 = v2.
   Proof.
     intros.
     dependent induction H;
@@ -244,8 +432,18 @@ Lemma ev_determ : forall t (e: exp nil t) v1 v2,
     assumption.
     assumption.
     assumption.
-    dependent destruction H.
-    rewrite 
-Qed.
+    dependent destruction H0.
+    apply IHEv in H0.
+    apply vconst_congS.
+    assumption.
+    dependent destruction H1.
+    rewrite (IHEv2 v3).
+    reflexivity.
+    rewrite (IHEv1 v2).
+    assumption.
+    assumption.
+    Admitted.
+  (* Need stronger IH with mutual induction *)
 
+  Check exp_ind.
   
